<?xml version="1.0"?>

<rdf:RDF xmlns="http://www.cgg.sm/ontology/cgg#"
    xml:base="http://www.cgg.sm/ontology/cgg#" 
    xmlns:rdf="http://www.w3.org/1999/02/22-rdf-syntax-ns#" 
    xmlns:rdfs="http://www.w3.org/2000/01/rdf-schema#" 
    xmlns:xsd="http://www.w3.org/2001/XMLSchema#" 
    xmlns:cggbase="http://www.cgg.sm/ontology/base#" 
    xmlns:cggtp="http://www.cgg.sm/ontology/textual-products#">

    <!-- GRAND AND GENERAL COUNCIL -->

    <rdfs:Class rdf:ID="GrandAndGeneralCouncil">
        <rdfs:label xml:lang="en">Grand and General Council</rdfs:label>
        <rdfs:label xml:lang="it">Consiglio Grande e Generale</rdfs:label>
        <rdfs:comment xml:lang="en">Institution responsible for the legislative power, the determination of political address and the exercise of control functions. Made up of 60 members called Councilors.</rdfs:comment>
        <rdfs:comment xml:lang="it">Istituzione alla quale spetta il potere legislativo, la determinazione dell’indirizzo politico e l’esercizio delle funzioni di controllo. È composto da 60 membri, chiamati Consiglieri.</rdfs:comment>
        <rdfs:subClassOf rdf:resource="http://www.cgg.sm/ontology/base#Institution"/>
    </rdfs:Class>

    <rdf:Property rdf:ID="debatesApprovesRejects">
        <rdfs:label xml:lang="en">debates, approves or rejects</rdfs:label>
        <rdfs:label xml:lang="it">dibatte, approva o rigetta</rdfs:label>
        <rdfs:comment xml:lang="en">Actions performable on norms by the Grand and General Council.</rdfs:comment>
        <rdfs:comment xml:lang="it">Azioni eseguibili sulle norme da parte del Consiglio Grande e Generale.</rdfs:comment>
        <rdfs:domain rdf:resource="#GrandAndGeneralCouncil"/>
        <rdfs:range rdf:resource="http://www.cgg.sm/ontology/textual-products#Norm"/>
    </rdf:Property>

    <rdfs:Class rdf:ID="Councilor">
        <rdfs:label xml:lang="en">Councilor</rdfs:label>
        <rdfs:label xml:lang="it">Consigliere</rdfs:label>
        <rdfs:comment xml:lang="en">One of the 60 members of the GGC, belonging to a political force or mixed group.</rdfs:comment>
        <rdfs:comment xml:lang="it">Uno dei 60 membri del CGG, appartenente ad una forza politica o al gruppo misto.</rdfs:comment>
        <rdfs:subClassOf rdf:resource="http://www.cgg.sm/ontology/base#Politician"/>
    </rdfs:Class>

    <rdf:Property rdf:ID="belongsToGroup">
        <rdfs:label xml:lang="en">belongs to Parliamentary Group</rdfs:label>
        <rdfs:label xml:lang="it">appartiene ad un Gruppo parlamentare</rdfs:label>
        <rdfs:comment xml:lang="en">Bond of membership of a Councilor to a Parliamentary Group.</rdfs:comment>
        <rdfs:comment xml:lang="it">Legame di appartenenza di un Consigliere ad un Gruppo parlamentare.</rdfs:comment>
        <rdfs:subPropertyOf rdf:resource="http://www.cgg.sm/ontology/base#belongsTo"/>
        <rdfs:domain rdf:resource="#Councilor"/>
        <rdfs:range rdf:resource="#ParliamentaryGroup"/>
    </rdf:Property>

    <rdf:Property rdf:ID="cggComposedBy">
        <rdfs:label xml:lang="en">GGC composed by</rdfs:label>
        <rdfs:label xml:lang="it">CGG composto da</rdfs:label>
        <rdfs:comment xml:lang="en">Composition of the GGC by Parliamentary Groups.</rdfs:comment>
        <rdfs:comment xml:lang="it">Composizione del CGG da parte di Gruppi parlamentari.</rdfs:comment>
        <rdfs:subPropertyOf rdf:resource="http://www.cgg.sm/ontology/base#composedBy"/>
        <rdfs:domain rdf:resource="#GrandAndGeneralCouncil"/>
        <rdfs:range rdf:resource="#ParliamentaryGroup"/>
    </rdf:Property>

    <rdfs:Class rdf:ID="ParliamentaryGroup">
        <rdfs:label xml:lang="en">Parliamentary Group</rdfs:label>
        <rdfs:label xml:lang="it">Gruppo parlamentare</rdfs:label>
        <rdfs:comment xml:lang="en">A parliamentary group is an organ that gathers the political demands and representations within a parliament.</rdfs:comment>
        <rdfs:comment xml:lang="it">Un gruppo parlamentare è un organo che raccoglie le istanze e le rappresentanze politiche all'interno di un parlamento.</rdfs:comment>
    </rdfs:Class>

    <rdf:Property rdf:ID="belongsToBloc">
        <rdfs:label xml:lang="en">belongs to a bloc</rdfs:label>
        <rdfs:label xml:lang="it">appartiene ad una fazione</rdfs:label>
        <rdfs:comment xml:lang="en">Bond of membership of a parliamentary group to a specific faction (majority or minority).</rdfs:comment>
        <rdfs:comment xml:lang="it">Appartenenza di un gruppo parlamentare ad una specifica fazione (maggioranza o minoranza).</rdfs:comment>
        <rdfs:subPropertyOf rdf:resource="#belongsTo"/>
        <rdfs:domain rdf:resource="#ParliamentaryGroup"/>
        <rdfs:range rdf:resource="#ParliamentaryBloc"/>
    </rdf:Property>

    <rdfs:Class rdf:ID="ParliamentaryBloc">
        <rdfs:label xml:lang="en">Parliamentary Bloc</rdfs:label>
        <rdfs:label xml:lang="it">Fazione parlamentare</rdfs:label>
        <rdfs:comment xml:lang="en">Partitioning of the Parliament in majority and minority.</rdfs:comment>
        <rdfs:comment xml:lang="it">Suddivisione del Parlamento in maggioranza e minoranza.</rdfs:comment>
    </rdfs:Class>

    <rdfs:Class rdf:ID="CounciliarGroup">
        <rdfs:label xml:lang="en">Counciliar Group</rdfs:label>
        <rdfs:label xml:lang="it">Gruppo Consiliare</rdfs:label>
        <rdfs:comment xml:lang="en">Delegation of a party within the GGC.</rdfs:comment>
        <rdfs:comment xml:lang="it">Rappresentanza parlamentare di un partito.</rdfs:comment>
        <rdfs:subClassOf rdf:resource="#ParliamentaryGroup"/>
    </rdfs:Class>

    <rdf:Property rdf:ID="headingTo">
        <rdfs:label xml:lang="en">heading to</rdfs:label>
        <rdfs:label xml:lang="it">facente capo a</rdfs:label>
        <rdfs:comment xml:lang="en">Link between the counciliar group and the party.</rdfs:comment>
        <rdfs:comment xml:lang="it">Collegamento tra il gruppo consiliare e il partito.</rdfs:comment>
        <rdfs:domain rdf:resource="#CounciliarGroup"/>
        <rdfs:range rdf:resource="#Party"/>
    </rdf:Property>

    <rdfs:Class rdf:ID="Party">
        <rdfs:label xml:lang="en">Party</rdfs:label>
        <rdfs:label xml:lang="it">Partito</rdfs:label>
        <rdfs:comment xml:lang="en">Association between people united by the same political purpose or by a common vision on fundamental issues of the management of the state and society or even only on specific and particular topics.</rdfs:comment>
        <rdfs:comment xml:lang="it">Associazione tra persone accomunate da una medesima finalità politica ovvero da una comune visione su questioni fondamentali della gestione dello Stato e della società o anche solo su temi specifici e particolari. </rdfs:comment>
    </rdfs:Class>

    <rdf:Property rdf:ID="name">
        <rdfs:label xml:lang="en">name</rdfs:label>
        <rdfs:label xml:lang="it">nome</rdfs:label>
        <rdfs:comment xml:lang="en">Name of the party.</rdfs:comment>
        <rdfs:comment xml:lang="it">Nome del partito.</rdfs:comment>
        <rdfs:domain rdf:resource="#Party"/>
        <rdfs:range rdf:resource="http://www.w3.org/2000/01/rdf-schema#Literal"/>
    </rdf:Property>

    <rdf:Property rdf:ID="contact">
        <rdfs:label xml:lang="en">contact</rdfs:label>
        <rdfs:label xml:lang="it">contatto</rdfs:label>
        <rdfs:comment xml:lang="en">Contact information of the party.</rdfs:comment>
        <rdfs:comment xml:lang="it">Informazioni di contatto del partito.</rdfs:comment>
        <rdfs:domain rdf:resource="#Party"/>
        <rdfs:range rdf:resource="http://www.cgg.sm/ontology/base#Contact"/>
    </rdf:Property>

    <rdfs:Class rdf:ID="Coalition">
        <rdfs:label xml:lang="en">Coalition</rdfs:label>
        <rdfs:label xml:lang="it">Coalizione</rdfs:label>
        <rdfs:comment xml:lang="en">Grouping of several counciliar groups.</rdfs:comment>
        <rdfs:comment xml:lang="it">Raggruppamento di più gruppi consiliari.</rdfs:comment>
    </rdfs:Class>

    <rdf:Property rdf:ID="coalitionComposedBy">
        <rdfs:label xml:lang="en">coalition composed by</rdfs:label>
        <rdfs:label xml:lang="it">coalizione composta da</rdfs:label>
        <rdfs:comment xml:lang="en">Grouping link of counciliar groups into coalitions.</rdfs:comment>
        <rdfs:comment xml:lang="it">Legame di raggruppamento di gruppi consiliari in coalizioni.</rdfs:comment>
        <rdfs:domain rdf:resource="#Coalition"/>
        <rdfs:range rdf:resource="#CounciliarGroup"/>
        <rdfs:subPropertyOf rdf:resource="#composedBy"/>
    </rdf:Property>

    <rdf:Property rdf:ID="leader">
        <rdfs:label xml:lang="en">Leader</rdfs:label>
        <rdfs:label xml:lang="it">Capogruppo</rdfs:label>
        <rdfs:comment xml:lang="en">A Councilor representing the Counciliar Group within the Parliament.</rdfs:comment>
        <rdfs:comment xml:lang="it">Un Consigliere che rappresenta il Gruppo Consiliare all'interno del Parlamento.</rdfs:comment>
        <rdfs:domain rdf:resource="#CounciliarGroup"/>
        <rdfs:range rdf:resource="#Councilor"/>
    </rdf:Property>

    <rdfs:Class rdf:ID="MixedGroup">
        <rdfs:label xml:lang="en">Mixed Group</rdfs:label>
        <rdfs:label xml:lang="it">Gruppo Misto</rdfs:label>
        <rdfs:comment xml:lang="en">A group of Independent Councilors.</rdfs:comment>
        <rdfs:comment xml:lang="it">Gruppo di Consiglieri indipendenti.</rdfs:comment>
        <rdfs:subClassOf rdf:resource="#ParliamentaryGroup"/>
    </rdfs:Class>

    <rdf:Property rdf:ID="electedFor">
        <rdfs:label xml:lang="en">elected for</rdfs:label>
        <rdfs:label xml:lang="it">eletto per</rdfs:label>
        <rdfs:comment xml:lang="en">Current Grand and General Council legislature.</rdfs:comment>
        <rdfs:comment xml:lang="it">Legislatura attuale del Consiglio Grande e Generale.</rdfs:comment>
        <rdfs:domain rdf:resource="#GrandAndGeneralCouncil"/>
        <rdfs:range rdf:resource="#Legislature"/>
    </rdf:Property>

    <rdfs:Class rdf:ID="Legislature">
        <rdfs:label xml:lang="en">Legislature</rdfs:label>
        <rdfs:label xml:lang="it">Legislatura</rdfs:label>
        <rdfs:comment xml:lang="en">Period of stay of the Grand and General Council.</rdfs:comment>
        <rdfs:comment xml:lang="it">Periodo di permanenza del Consiglio Grande e Generale.</rdfs:comment>
    </rdfs:Class>

    <rdf:Property rdf:ID="begins">
        <rdfs:label xml:lang="en">start date</rdfs:label>
        <rdfs:label xml:lang="it">data di inizio</rdfs:label>
        <rdfs:comment xml:lang="en">Start date of the Legislature.</rdfs:comment>
        <rdfs:comment xml:lang="it">Data di inizio della Legislature.</rdfs:comment>
        <rdfs:domain rdf:resource="#Legislature"/>
        <rdfs:range rdf:resource="http://www.w3.org/2001/XMLSchema#date"/>
    </rdf:Property>

    <rdf:Property rdf:ID="ends">
        <rdfs:label xml:lang="en">end date</rdfs:label>
        <rdfs:label xml:lang="it">data di fine</rdfs:label>
        <rdfs:comment xml:lang="en">End date of the Legislature.</rdfs:comment>
        <rdfs:comment xml:lang="it">Data di fine della Legislature.</rdfs:comment>
        <rdfs:domain rdf:resource="#Legislature"/>
        <rdfs:range rdf:resource="http://www.w3.org/2001/XMLSchema#date"/>
    </rdf:Property>

</rdf:RDF>