<?xml version="1.0"?>

<rdf:RDF xmlns="http://www.cgg.sm/ontology/council-of-12#"
  xml:base="http://www.cgg.sm/ontology/council-of-12#"
  xmlns:rdf="http://www.w3.org/1999/02/22-rdf-syntax-ns#" 
  xmlns:rdfs="http://www.w3.org/2000/01/rdf-schema#" 
  xmlns:cggroot="http://www.cgg.sm/ontology/cgg#" 
  xmlns:cggbase="http://www.cgg.sm/ontology/cgg#">

  <!-- COUNCIL OF 12 -->

  <rdfs:Class rdf:ID="CouncilOfTwelves">
    <rdfs:label xml:lang="en">Council of Twelves</rdfs:label>
    <rdfs:label xml:lang="it">Consiglio dei XII</rdfs:label>
    <rdfs:comment xml:lang="en">Institutional body of the Republic of San Marino to which administrative functions are assigned.</rdfs:comment>
    <rdfs:comment xml:lang="it">Organo istituzionale della Repubblica di San Marino cui sono attribuite funzioni amministrative. </rdfs:comment>
    <rdfs:subClassOf rdf:resource="http://www.cgg.sm/ontology/base#Institution"/>
  </rdfs:Class>

  <rdf:Property rdf:ID="composedByCouncilors">
    <rdfs:label xml:lang="en">composed by Councilors</rdfs:label>
    <rdfs:label xml:lang="it">composto da Consiglieri</rdfs:label>
    <rdfs:comment xml:lang="en">Composition of the Council of Twelves by Councilors.</rdfs:comment>
    <rdfs:comment xml:lang="it">Composizione del Consiglio dei Dodici da parte di Consiglieri.</rdfs:comment>
    <rdfs:subPropertyOf rdf:resource="http://www.cgg.sm/ontology/base#composedBy"/>
    <rdfs:domain rdf:resource="#CouncilOfTwelves"/>
    <rdfs:range rdf:resource="http://www.cgg.sm/ontology/cgg#Councilor"/>
  </rdf:Property>

  <rdf:Property rdf:ID="functionsOfCouncilOfTwelves">
    <rdfs:label xml:lang="en">functions of the Council of Twelves</rdfs:label>
    <rdfs:label xml:lang="it">funzioni del Consiglio dei Dodici</rdfs:label>
    <rdfs:comment xml:lang="en">Functions assigned to the Council of Twelves.</rdfs:comment>
    <rdfs:comment xml:lang="it">Funzioni assegnate al Consiglio dei Dodici.</rdfs:comment>
    <rdfs:subPropertyOf rdf:resource="http://www.cgg.sm/ontology/base#functions"/>
    <rdfs:domain rdf:resource="#CouncilOfTwelves"/>
    <rdfs:range rdf:resource="http://www.w3.org/2000/01/rdf-schema#Literal"/>
  </rdf:Property>

</rdf:RDF>