<?xml version="1.0"?>

<rdf:RDF xmlns="http://www.cgg.sm/ontology/international-delegations#"
    xml:base="http://www.cgg.sm/ontology/international-delegations#"
    xmlns:rdf="http://www.w3.org/1999/02/22-rdf-syntax-ns#" 
    xmlns:rdfs="http://www.w3.org/2000/01/rdf-schema#" 
    xmlns:cggbase="http://www.cgg.sm/ontology/base#" 
    xmlns:cggroot="http://www.cgg.sm/ontology/cgg#">

    <!-- INTERNATIONAL DELEGATIONS -->

    <rdfs:Class rdf:ID="CounciliarDelegationAtInternationalOrganizations">
        <rdfs:label xml:lang="en">Counciliar Delegation at International Organization</rdfs:label>
        <rdfs:label xml:lang="it">Delegazione Consiliare presso Organismo Internazionale</rdfs:label>
        <rdfs:comment xml:lang="en">Counciliar delegation elected at the international organizations in order to represent the Republic.</rdfs:comment>
        <rdfs:comment xml:lang="it">Delegazioni consiliari elette presso le organizzazioni internazionali al fine di rappresentare la Repubblica.</rdfs:comment>
    </rdfs:Class>

    <rdf:Property rdf:ID="organizationName">
        <rdfs:label xml:lang="en">organization name</rdfs:label>
        <rdfs:label xml:lang="it">nome dell'organizzazione</rdfs:label>
        <rdfs:comment xml:lang="en">Name of the international organization.</rdfs:comment>
        <rdfs:comment xml:lang="it">Nome dell'organizzazione internazionale. </rdfs:comment>
        <rdfs:domain rdf:resource="#CounciliarDelegationAtInternationalOrganizations"/>
        <rdfs:range rdf:resource="http://www.w3.org/2000/01/rdf-schema#Literal"/>
    </rdf:Property>

    <rdf:Property rdf:ID="composedByDelegates">
        <rdfs:label xml:lang="en">composed by delegates</rdfs:label>
        <rdfs:label xml:lang="it">composta da delegati</rdfs:label>
        <rdfs:comment xml:lang="en">Composition of the delegation by delegated councilors.</rdfs:comment>
        <rdfs:comment xml:lang="it">Composizione della delegazione da parte di consiglieri delegati. </rdfs:comment>
        <rdfs:subPropertyOf rdf:resource="http://www.cgg.sm/ontology/base#composedBy"/>
        <rdfs:domain rdf:resource="#CounciliarDelegationAtInternationalOrganizations"/>
        <rdfs:range rdf:resource="#Delegated"/>
    </rdf:Property>

    <rdfs:Class rdf:ID="Delegated">
        <rdfs:label xml:lang="en">Delegated</rdfs:label>
        <rdfs:label xml:lang="it">Delegato</rdfs:label>
        <rdfs:comment xml:lang="en">A Councilor that takes part to the delegation for an International Organization.</rdfs:comment>
        <rdfs:comment xml:lang="it">Un Consigliere che prende parte alla delegazione per un'Organizzazione Internazionale. </rdfs:comment>
        <rdfs:subClassOf rdf:resource="http://www.cgg.sm/ontology/cgg#Councilor"/>
    </rdfs:Class>

    <rdfs:Class rdf:ID="HeadOfDelegation">
        <rdfs:label xml:lang="en">Head of Delegation</rdfs:label>
        <rdfs:label xml:lang="it">Capo delegazione</rdfs:label>
        <rdfs:comment xml:lang="en">The president of the delegation.</rdfs:comment>
        <rdfs:comment xml:lang="it">Il presidente della delegazione. </rdfs:comment>
        <rdfs:subClassOf rdf:resource="#Delegated"/>
    </rdfs:Class>

    <rdf:Property rdf:ID="functionsOfDelegation">
        <rdfs:label xml:lang="en">functions of the delegation</rdfs:label>
        <rdfs:label xml:lang="it">funzioni della delegazione</rdfs:label>
        <rdfs:comment xml:lang="en">A list of functions assigned to the delegation.</rdfs:comment>
        <rdfs:comment xml:lang="it">Una lista di funzioni assegnate alla delegazione. </rdfs:comment>
        <rdfs:subPropertyOf rdf:resource="http://www.cgg.sm/ontology/base#functions"/>
        <rdfs:domain rdf:resource="#CounciliarDelegationAtInternationalOrganizations"/>
        <rdfs:range rdf:resource="http://www.w3.org/2000/01/rdf-schema#Literal"/>
    </rdf:Property>

    <rdf:Property rdf:ID="annualReport">
        <rdfs:label xml:lang="en">annual report</rdfs:label>
        <rdfs:label xml:lang="it">relazione annuale</rdfs:label>
        <rdfs:comment xml:lang="en">The annual report about the activities of the delegation.</rdfs:comment>
        <rdfs:comment xml:lang="it">La relazione annuale relativa alle attivit√† svolte dalla delegazione. </rdfs:comment>
        <rdfs:domain rdf:resource="#CounciliarDelegationAtInternationalOrganizations"/>
        <rdfs:range rdf:resource="http://www.w3.org/2000/01/rdf-schema#Literal"/>
    </rdf:Property>

</rdf:RDF>